Flapjack/Test/SpillCosts.lean
@@ -17,6 +17,10 @@ example :
   decide
 
 example :
+    wordRaChooseSpillNodeByDegree [(3, 2), (5, 5), (7, 4)] 3 [5, 7] = 5 := by
+  decide
+
+example :
     wordRaChooseSpillNode [(3, 100), (5, 20), (7, 30)] [(3, 10), (5, 1), (7, 2)] 3 [5, 7] = 3 := by
   decide
 
